Tests/Base/TestIx.lean
@@ -10,12 +10,12 @@ def tests : List TestResult :=
     checkEq "Ix Nat range [3,7]" [3, 4, 5, 6, 7] (Ix.range (3, 7))
   , checkEq "Ix Nat range [5,5]" [5] (Ix.range (5, 5))
   , checkEq "Ix Nat range [5,3] empty" ([] : List Nat) (Ix.range (5, 3))
-  -- Nat index
-  , checkEq "Ix Nat index (3,7) 5" (some 2) (Ix.index (3, 7) 5)
-  , checkEq "Ix Nat index (3,7) 3" (some 0) (Ix.index (3, 7) 3)
-  , checkEq "Ix Nat index (3,7) 7" (some 4) (Ix.index (3, 7) 7)
-  , checkEq "Ix Nat index (3,7) 8 out" (none : Option Nat) (Ix.index (3, 7) 8)
-  , checkEq "Ix Nat index (3,7) 2 out" (none : Option Nat) (Ix.index (3, 7) 2)
+  -- Nat index (now returns Option {n : Nat // n < rangeSize bounds})
+  , checkEq "Ix Nat index (3,7) 5" (some 2) ((Ix.index (3, 7) 5).map (·.val))
+  , checkEq "Ix Nat index (3,7) 3" (some 0) ((Ix.index (3, 7) 3).map (·.val))
+  , checkEq "Ix Nat index (3,7) 7" (some 4) ((Ix.index (3, 7) 7).map (·.val))
+  , checkEq "Ix Nat index (3,7) 8 out" (none : Option Nat) ((Ix.index (3, 7) (8 : Nat)).map (·.val))
+  , checkEq "Ix Nat index (3,7) 2 out" (none : Option Nat) ((Ix.index (3, 7) (2 : Nat)).map (·.val))
   -- Nat inRange
   , check "Ix Nat inRange (3,7) 5" (Ix.inRange (3, 7) 5)
   , check "Ix Nat inRange (3,7) 3" (Ix.inRange (3, 7) 3)
@@ -28,8 +28,8 @@ def tests : List TestResult :=
   , checkEq "Ix Char range ('a','f')" ['a', 'b', 'c', 'd', 'e', 'f'] (Ix.range ('a', 'f'))
   , checkEq "Ix Char range ('a','a')" ['a'] (Ix.range ('a', 'a'))
   -- Char index
-  , checkEq "Ix Char index ('a','f') 'c'" (some 2) (Ix.index ('a', 'f') 'c')
-  , checkEq "Ix Char index ('a','f') 'z' out" (none : Option Nat) (Ix.index ('a', 'f') 'z')
+  , checkEq "Ix Char index ('a','f') 'c'" (some 2) ((Ix.index ('a', 'f') 'c').map (·.val))
+  , checkEq "Ix Char index ('a','f') 'z' out" (none : Option Nat) ((Ix.index ('a', 'f') 'z').map (·.val))
   -- Char inRange
   , check "Ix Char inRange ('a','f') 'd'" (Ix.inRange ('a', 'f') 'd')
   , check "Ix Char not inRange ('a','f') 'z'" (!Ix.inRange ('a', 'f') 'z')
@@ -39,11 +39,11 @@ def tests : List TestResult :=
   , checkEq "Ix Bool range (true,true)" [true] (Ix.range (true, true))
   , checkEq "Ix Bool range (true,false) empty" ([] : List Bool) (Ix.range (true, false))
   -- Bool index
-  , checkEq "Ix Bool index (false,true) true" (some 1) (Ix.index (false, true) true)
-  , checkEq "Ix Bool index (false,true) false" (some 0) (Ix.index (false, true) false)
+  , checkEq "Ix Bool index (false,true) true" (some 1) ((Ix.index (false, true) true).map (·.val))
+  , checkEq "Ix Bool index (false,true) false" (some 0) ((Ix.index (false, true) false).map (·.val))
   -- Int range
   , checkEq "Ix Int range (-2,2)" ([-2, -1, 0, 1, 2] : List Int) (Ix.range ((-2 : Int), 2))
-  , checkEq "Ix Int index (-2,2) 0" (some 2) (Ix.index ((-2 : Int), (2 : Int)) (0 : Int))
+  , checkEq "Ix Int index (-2,2) 0" (some 2) ((Ix.index ((-2 : Int), (2 : Int)) (0 : Int)).map (·.val))
   -- Proof coverage
   , proofCovered "Ix.inRange_iff_index_isSome_nat" "Hale.Base.Data.Ix"
   ]
